Finished the CRC32 checksum.

code/c/Yazi_CRC32_Table_Codegen.c
@@ -6,6 +6,9 @@ int main(int argc, const char **argv) {
   uint32_t table[4][256];
   gen_crc32_table(table[0], table[1], table[2], table[3]);
 
+  uint32_t matrix[32];
+  gen_matrix_table(matrix);
+
   printf("static uint32_t crc32_table[4][256] = {\n");
   
   for (int i = 0; i < 4; i++) {
@@ -25,12 +28,56 @@ int main(int argc, const char **argv) {
       printf(", ");
     }
   }
-  
+
   printf(
     "\n};\n\n"
+    "uint32_t crc32_combine64(uint32_t crc1, uint32_t crc2, uint64_t len2) {\n"
+    "  uint32_t m0[32];\n"
+    "  uint32_t m1[32] = {\n");
+
+  for (int i = 0; i < 32; i++) {
+    printf("0x%.8xUL, ", matrix[i]);
+    if (i > 0 && i % 5 == 0) {
+      printf("\n  ");
+    }
+  }
+  
+  printf(
+    "  \n};\n"
+    "  if (len2 == 0) {\n"
+    "    return crc1;\n"
+    "  }\n\n"
+    "  for (;;) {\n"
+    "    if (len2 & 1) {\n"
+    "      crc1 = Yazi_CRC32_Impl_gf2_matrix_times((uint32_t *)m1, crc1);\n"
+    "    }\n\n"
+    "    len2 >>= 1;\n"
+    "    if (len2 > 0) {\n"
+    "      Yazi_CRC32_Impl_gf2_matrix_square((uint32_t *)m1, (uint32_t *)m0);\n"
+    "      if (len2 & 1) {\n"
+    "        crc1 = Yazi_CRC32_Impl_gf2_matrix_times((uint32_t *)m0, crc1);\n"
+    "      }\n"
+    "      len2 >>= 1;\n"
+    "      if (len2 > 0) {\n"
+    "        Yazi_CRC32_Impl_gf2_matrix_square((uint32_t *)m0, (uint32_t *)m1);\n"
+    "      } else {\n"
+    "        break;\n"
+    "      }\n"
+    "    } else {\n"
+    "      break;\n"
+    "    }\n"
+    "  }\n\n"
+    "  return crc1 ^ crc2;\n}\n\n"
+    "uint32_t crc32_combine(uint32_t crc1, uint32_t crc2, uint32_t len2) {\n"
+    "  return crc32_combine64(crc1, crc2, len2);\n"
+    "}\n\n"
     "unsigned int crc32(unsigned int crc, const unsigned char *buf, unsigned int len) {\n"
-    "  return Yazi_CRC32_crc32_impl((uint32_t *)crc32_table, crc, len, (uint8_t *) buf);\n"
+    "  return Yazi_CRC32_Impl_crc32_impl((uint32_t *)crc32_table, crc, len, (uint8_t *) buf);\n"
     "}\n");
 
   return 0;
 }
+
+static uint32_t m1[32] = {0};
+
+
