specs/Spec.CRC32.Matrix.fst
@@ -1,170 +1,81 @@
 module Spec.CRC32.Matrix
 
+module B = LowStar.Buffer
 module BV = FStar.BitVector
 module Bits = Spec.CRC32.Bits
+module HS = FStar.HyperStack
 module Seq = FStar.Seq
+module U32 = FStar.UInt32
+module UInt = FStar.UInt
 
-open FStar.Seq
-open FStar.Mul
-open Spec.CRC32.Bits
+let magic_matrix_pattern (nzeros: nat{nzeros > 0}) (i: nat{i < 32}):
+  res: BV.bv_t (nzeros + 32){
+    forall j.
+      (j == nzeros + 31 - i ==> Seq.index res j == true) /\
+      (j <> nzeros + 31 - i ==> Seq.index res j == false)
+  } =
+  let zero_left = BV.zero_vec #(nzeros + 32 - i - 1) in
+  let one = Bits.ones_vec_r 1 zero_left in
+  Bits.zero_vec_r i one
 
-#set-options "--z3rlimit 200 --fuel 1 --ifuel 1"
-let rec seq_append_index_r (#t: Type) (a b: Seq.seq t): Lemma
-  (ensures forall i. i < Seq.length b ==> Seq.index (a @| b) (i + Seq.length a) == Seq.index b i)
-  (decreases Seq.length a) =
-  match Seq.length a with
-  | 0 -> ()
-  | _ -> seq_append_index_r (Seq.tail a) b
+unfold let is_magic_matrix_elem (nzeros: nat{nzeros > 0}) (i: nat {i < 32}) (v: BV.bv_t 32) =
+  Bits.poly_mod (magic_matrix_pattern nzeros i) == v
 
-val magic_matrix_init: s: sub_matrix_t 1 -> Tot (matrix_t 1) (decreases 32 - (Seq.length s))
+unfold let is_sub_matrix_buf
+  (h: HS.mem)
+  (len: nat{len <= 32})
+  (nzeros: nat{nzeros > 0})
+  (buf: B.buffer U32.t{B.length buf == 32}) =
+  B.live h buf /\
+  (forall (i: nat{i < len}).
+    is_magic_matrix_elem nzeros i (UInt.to_vec (U32.v (Seq.index (B.as_seq h buf) i))))
 
-let rec magic_matrix_init s =
-  let l = Seq.length s in
-  if l = 0 then begin
-    let m = ones_vec_r 1 (BV.zero_vec #32) in
-    let n = poly_xor (BV.zero_vec #32) in
-    calc (==) {
-      poly_mod #33 m;
-      =={assert(last m == true)}
-      unsnoc (m -@ poly 33);
-      =={}
-      n;
-    };
-    let res = s @| (Seq.create 1 n) in
-    assert(Seq.length res == l + 1);
-    calc (==) {
-      Seq.index res l;
-      =={seq_append_index_r s (Seq.create 1 n)}
-      Seq.index (Seq.create 1 n) 0;
-      =={}
-      n;
-    };
-    magic_matrix_init res
-  end else if l < 32 then begin
-    let n = magic_matrix_pattern 1 l in
-    let res = s @| (Seq.create 1 (poly_mod n)) in
-    calc (==) {
-      Seq.index res l;
-      =={seq_append_index_r s (Seq.create 1 (poly_mod n))}
-      poly_mod n;
-    };
-    magic_matrix_init res
-  end else 
-    s
+unfold let is_matrix_buf
+  (h: HS.mem)
+  (nzeros: nat{nzeros > 0})
+  (buf: B.buffer U32.t{B.length buf == 32}) = is_sub_matrix_buf h 32 nzeros buf
 
-val do_magic_matrix_times:
-    #nzeros: nat{nzeros > 0}
-  -> m: matrix_t nzeros
-  -> n: BV.bv_t 32
-  -> i: nat{i < 32}
-  -> res: BV.bv_t 32{
-      res == poly_mod (bit_extract #nzeros (zero_vec_l nzeros n) i)
-    }
-
-let do_magic_matrix_times #nzeros m n i =
-  let pat = magic_matrix_pattern nzeros i in
-  let ext = bit_extract #nzeros (zero_vec_l nzeros n) i in
-  if Seq.index n (31 - i) then begin
-    assert(Seq.equal (magic_matrix_pattern nzeros i) (ext));
-    Seq.index m i
-  end else begin
-    assert(Seq.equal ext (BV.zero_vec #(nzeros + 32)));
-    Bits.poly_mod_zero ext;
-    BV.zero_vec #32
-  end
-
-val magic_matrix_times':
-    #nzeros: nat{nzeros > 0}
-  -> m: matrix_t nzeros
-  -> n: BV.bv_t 32
-  -> i: nat{i < 32}
-  -> res: BV.bv_t 32{
-    res == poly_mod (bit_sum #nzeros (zero_vec_l nzeros n) i)
-  }
-
-let rec magic_matrix_times'
-  (#nzeros: nat{nzeros > 0}) (m: matrix_t nzeros) (n: BV.bv_t 32) (i: nat{i < 32}) =
+let bit_extract
+  (#len: nat{len > 0})
+  (n: BV.bv_t len)
+  (i: nat{0 <= i /\ i <= len - 1}):
+  Tot (res: BV.bv_t len {
+    forall j.
+      (j == len - i - 1 ==> Seq.index res j == Seq.index n j) /\
+      (j <> len - i - 1 ==> Seq.index res j == false)
+  }) =
+  let zero_left = if i = len - 1 then Seq.empty #bool else BV.zero_vec #(len - i - 1) in
+  let bit = Seq.snoc zero_left (Seq.index n (len - i - 1)) in
+  Bits.zero_vec_r #(len - i) i bit
+  
+let rec bit_sum
+  (#len: nat{len > 0})
+  (n: BV.bv_t len)
+  (i: nat{0 <= i /\ i <= len - 1}):
+  Tot (res: BV.bv_t len {
+    forall j.
+      (j >= len - i - 1 ==> Seq.index res j == Seq.index n j) /\
+      (j < len - i - 1 ==> Seq.index res j == false)
+  }) =
   match i with
-  | 0 -> do_magic_matrix_times m n i
-  | _ -> 
-    let n' = do_magic_matrix_times m n i in
-    let e = bit_extract #nzeros (zero_vec_l nzeros n) i in
-    let sum = bit_sum #nzeros (zero_vec_l nzeros n) (i - 1) in
-    Bits.poly_mod_add e sum;
-    n' +@ magic_matrix_times' m n (i - 1)
+  | 0 -> bit_extract n i
+  | _ -> Bits.gf2_plus (bit_extract n i) (bit_sum n (i - 1))
 
-val magic_matrix_times:
-  #nzeros: nat {nzeros > 0} ->
-  matrix_t nzeros ->
-  n: BV.bv_t 32 ->
-  res: BV.bv_t 32 {res == poly_mod (zero_vec_l nzeros n)}
+let bit_extract_eq_pattern
+  (#len: nat{len > 32})
+  (n: BV.bv_t len)
+  (i: nat{i < 32}): Lemma
+  (requires Seq.index n (len - 1 - i) == true)
+  (ensures bit_extract n i == magic_matrix_pattern (len - 32) i) =
+  assert(Seq.equal (bit_extract n i) (magic_matrix_pattern (len - 32) i))
 
-let magic_matrix_times #nzeros m n =
-  assert(Seq.equal (bit_sum #nzeros (zero_vec_l nzeros n) 31) (zero_vec_l nzeros n));
-  magic_matrix_times' m n 31
-
-let magic_matrix_times_double
-  (#nzeros: nat{nzeros > 0}) (m: matrix_t nzeros) (i: nat{i < 32}): Lemma
-  (ensures is_magic_matrix_elem (nzeros * 2) i (magic_matrix_times m (Seq.index m i))) =
-  let p = magic_matrix_pattern nzeros i in
-  let p' = magic_matrix_pattern (nzeros * 2) i in
-  let p'' = zero_vec_l nzeros p in
-  let n = magic_matrix_times m (Seq.index m i) in
-  poly_mod_zero_prefix p nzeros;
-  assert(forall j.
-    j >= nzeros /\ j < nzeros * 2 + 32 ==>
-    Seq.index p (j - nzeros) == Seq.index p' j /\
-    Seq.index p (j - nzeros) == Seq.index p'' j);
-  assert(forall j. j < nzeros ==> Seq.index p' j == Seq.index p'' j);
-  assert(Seq.equal p'' p');
-  calc (==) {
-    n;
-    =={}
-    poly_mod (zero_vec_l nzeros (Seq.index m i));
-    =={}
-    poly_mod (zero_vec_l nzeros (poly_mod p));
-    =={}
-    poly_mod (zero_vec_l nzeros p);
-    =={}
-    poly_mod p';
-    =={}
-    poly_mod (magic_matrix_pattern (nzeros * 2) i);
+type sub_matrix_times_product (nzeros: nat{nzeros > 0}) (i: nat{i < 32}) (vec: U32.t) = 
+  res: U32.t{
+    let vec' = Bits.zero_vec_l nzeros (UInt.to_vec (U32.v vec)) in
+    UInt.to_vec (U32.v res) == Bits.poly_mod (bit_sum vec' i)
   }
 
-val magic_matrix_square':
-    #nzeros: nat{nzeros > 0}
-  -> m: matrix_t nzeros
-  -> s: sub_matrix_t (nzeros * 2)
-  -> Tot (matrix_t (nzeros * 2))
-    (decreases 32 - (Seq.length s))
+type matrix_times_product (nzeros: nat{nzeros > 0}) (vec: U32.t) =
+  sub_matrix_times_product nzeros 31 vec
 
-let rec magic_matrix_square' #nzeros m s =
-  if Seq.length s < 32 then begin
-    magic_matrix_times_double m (Seq.length s);
-    let n = magic_matrix_times m (Seq.index m (Seq.length s)) in
-    let res = s @| (Seq.create 1 n) in
-    seq_append_index_r s (Seq.create 1 n);
-    calc (==) {
-      poly_mod (magic_matrix_pattern (nzeros * 2) (Seq.length s));
-      =={}
-      n;
-      =={}
-      Seq.index (Seq.create 1 n) 0;
-      =={}
-      Seq.index res (Seq.length s);
-    };
-    assert(forall i.{:pattern Seq.index res i}
-      i < Seq.length s ==> Seq.index res i == Seq.index s i);
-    assert(forall i. i < Seq.length res ==> is_magic_matrix_elem (nzeros * 2) i (Seq.index res i));
-    magic_matrix_square' #nzeros m res
-  end
-  else
-    s
-
-val magic_matrix_square:
-    #nzeros: nat {nzeros > 0}
-  -> matrix_t nzeros
-  -> Tot (matrix_t (nzeros * 2))
-
-let magic_matrix_square #_ m =
-  magic_matrix_square' m (Seq.empty #(BV.bv_t 32))
+type matrix_buf = m: B.buffer U32.t{B.length m == 32}
